

Задача 6

Упростить выражение $x = (B \rightarrow A) \cdot \overline{(A + B)} \cdot (A \rightarrow C)$

$$\begin{aligned} x &= (B \rightarrow A) \cdot \overline{(A + B)} \cdot (A \rightarrow C) = (!B + A) \cdot !A \cdot !B \cdot (!A + C) = \\ &= (!A \cdot !B + A \cdot !A) \cdot !B \cdot (!A + C) = \\ &= (!A \cdot !B + 0) \cdot !B \cdot (!A + C) = !A \cdot !B \cdot !B \cdot (!A + C) = \\ &= !A \cdot !B \cdot (!A + C) = !A \cdot !B \cdot !A + !A \cdot !B \cdot C = \\ &= !A \cdot !B \cdot (1 + C) = !A \cdot !B \cdot 1 = !A \cdot !B \end{aligned}$$

Отв. $x = !A \cdot !B$